io/case-study/WebServer.fst
@@ -15,11 +15,11 @@ type req_handler (fl:erased tflag) =
   (req:Bytes.bytes) ->
   (send:(res:Bytes.bytes -> MIO (resexn unit) mymst fl (requires (fun h -> did_not_respond h /\ valid_http_response res))
                                             (ensures (fun _ _ lt -> exists r. lt == [EWrite Prog (client,res) r] /\
-                                                                  wrote_at_least_once_to client lt)))) ->
+                                                                  wrote_to client lt)))) ->
   MIO (resexn unit) mymst fl
     (requires (fun h -> valid_http_request req /\ did_not_respond h))
     (ensures (fun h r lt -> enforced_locally pi h lt /\
-                          (wrote_at_least_once_to client lt \/ Inr? r)))
+                          (wrote_to client lt \/ Inr? r)))
 
 let static_cmd
   (cmd : io_cmds)
@@ -58,9 +58,9 @@ let process_connection
     introduce enforced_locally pi h lthandler /\ every_request_gets_a_response (lt @ lt') ==> every_request_gets_a_response (lt @ lthandler @ lt')
     with _. ergar_pi_irr h lthandler lt lt'
   end ;
-  introduce forall h lthandler client limit r lt. enforced_locally pi h lthandler /\ wrote_at_least_once_to client lthandler /\ every_request_gets_a_response lt ==> every_request_gets_a_response (lt @ [ ERead Prog (client, limit) (Inl r) ] @ lthandler)
+  introduce forall h lthandler client limit r lt. enforced_locally pi h lthandler /\ wrote_to client lthandler /\ every_request_gets_a_response lt ==> every_request_gets_a_response (lt @ [ ERead Prog (client, limit) (Inl r) ] @ lthandler)
   with begin
-    introduce enforced_locally pi h lthandler /\ wrote_at_least_once_to client lthandler /\ every_request_gets_a_response lt ==> every_request_gets_a_response (lt @ [ ERead Prog (client, limit) (Inl r) ] @ lthandler)
+    introduce enforced_locally pi h lthandler /\ wrote_to client lthandler /\ every_request_gets_a_response lt ==> every_request_gets_a_response (lt @ [ ERead Prog (client, limit) (Inl r) ] @ lthandler)
     with _. ergar_pi_write h lthandler client limit r lt
   end ;
   match get_req client with
@@ -178,7 +178,7 @@ let webserver
 let check_send_pre : tree (pck_dc mymst) =
   Node
     (| Bytes.bytes, unit, (fun res h _ _ ->
-      Utils.did_not_respond' h && valid_http_response res), (fun res s0 _ _ -> s0.waiting && valid_http_response res) |)
+      Utils.did_not_respond h && valid_http_response res), (fun res s0 _ _ -> s0.waiting && valid_http_response res) |)
     Leaf
     Leaf
 
@@ -191,7 +191,7 @@ let check_handler_post : tree (pck_dc mymst) =
   Node (|
     file_descr,
     unit,
-    (fun client _ _ lt -> Utils.wrote_at_least_once_to' client lt),
+    (fun client _ _ lt -> Utils.wrote_to client lt),
     (fun client s0 _ s1 -> client `List.mem` s1.written)
     |)
     check_send_pre
